code/experimental/rsa/Hacl.Impl.MGF.fst
@@ -12,69 +12,68 @@ open Hacl.Impl.Convert
 module Buffer = Spec.Lib.IntBuf
 
 (* SHA 256 *)
-inline_for_extraction 
+inline_for_extraction
 let hLen:size_t = size 32
 
 assume val hash_sha256:
-    #len:size_nat ->
-    mHash:lbytes (v hLen) ->
-    clen:size_t{v clen == len} ->
-    m:lbytes len -> Stack unit
-    (requires (fun h -> live h mHash /\ live h m /\ disjoint m mHash))
-    (ensures (fun h0 _ h1 -> preserves_live h0 h1 /\ modifies1 mHash h0 h1))
+  #len:size_nat ->
+  mHash:lbytes (v hLen) ->
+  clen:size_t{v clen == len} ->
+  m:lbytes len -> Stack unit
+  (requires (fun h -> live h mHash /\ live h m /\ disjoint m mHash))
+  (ensures (fun h0 _ h1 -> preserves_live h0 h1 /\ modifies1 mHash h0 h1))
 //let hash_sha256 #len mHash clen m = SHA2_256.hash mHash m clen
 
 (* Mask Generation Function *)
 val mgf_sha256_:
-    count_max:size_t ->
-    accLen:size_t{v accLen = v hLen * v count_max} ->
-    stLen:size_t{v stLen = 4 + 2 * v hLen + v accLen} -> st:lbytes (v stLen) ->
-    counter:size_t{v counter <= v count_max} -> Stack unit
-    (requires (fun h -> live h st))
-    (ensures (fun h0 _ h1 -> preserves_live h0 h1 /\ modifies1 st h0 h1))
-    #reset-options "--z3rlimit 50 --max_fuel 0 --max_ifuel 0"
-    [@"c_inline"]
-let rec mgf_sha256_ count_max accLen stLen st counter =
-  if (counter <. count_max) then begin
-     let mgfseed_counter_len = add #SIZE hLen (size 4) in
-     let mgfseed_counter = Buffer.sub #uint8 #(v stLen) #(v mgfseed_counter_len) st (size 0) mgfseed_counter_len in
-     let mHash = Buffer.sub #uint8 #(v stLen) #(v hLen) st mgfseed_counter_len hLen in
-     let acc = Buffer.sub #uint8 #(v stLen) #(v accLen) st (add #SIZE mgfseed_counter_len hLen) accLen in
-     let c = Buffer.sub #uint8 #(v mgfseed_counter_len) #4 mgfseed_counter hLen (size 4) in
-     c.(size 0) <- to_u8 #U32 (size_to_uint32 counter >>. u32 24);
-     c.(size 1) <- to_u8 #U32 (size_to_uint32 counter >>. u32 16);
-     c.(size 2) <- to_u8 #U32 (size_to_uint32 counter >>. u32 8);
-     c.(size 3) <- to_u8 #U32 (size_to_uint32 counter);
+  #stLen:size_nat -> mgfseedLen:size_t -> accLen:size_t ->
+  sstLen:size_t{v sstLen = stLen /\ stLen = v mgfseedLen + 4 + v hLen + v accLen} ->
+  st:lbytes stLen -> count_max:size_t{v accLen = v count_max * v hLen} -> Stack unit
+  (requires (fun h -> live h st))
+  (ensures (fun h0 _ h1 -> preserves_live h0 h1 /\ modifies1 st h0 h1))
+  [@"c_inline"]
+let mgf_sha256_ #stLen mgfseedLen accLen sstLen st count_max =
+  iteri_simple #uint8 #stLen count_max
+  (fun counter st ->
+    let mgfseed_counterLen = add #SIZE mgfseedLen (size 4) in
+    let mgfseed_counter = Buffer.sub #uint8 #stLen #(v mgfseed_counterLen) st (size 0) mgfseed_counterLen in
+    let mHash = Buffer.sub #uint8 #stLen #(v hLen) st mgfseed_counterLen hLen in
+    let acc = Buffer.sub #uint8 #stLen #(v accLen) st (add #SIZE mgfseed_counterLen hLen) accLen in
+    let c = Buffer.sub #uint8 #(v mgfseed_counterLen) #4 mgfseed_counter mgfseedLen (size 4) in
 
-     hash_sha256 mHash mgfseed_counter_len mgfseed_counter;
-     let acc' = Buffer.sub #uint8 #(v accLen) #(v hLen) acc (mul #SIZE hLen counter) hLen in
-     copy hLen mHash acc';
-     mgf_sha256_ count_max accLen stLen st (add #SIZE counter (size 1))
-  end
+    c.(size 0) <- to_u8 #U32 (size_to_uint32 counter >>. u32 24);
+    c.(size 1) <- to_u8 #U32 (size_to_uint32 counter >>. u32 16);
+    c.(size 2) <- to_u8 #U32 (size_to_uint32 counter >>. u32 8);
+    c.(size 3) <- to_u8 #U32 (size_to_uint32 counter);
+
+    hash_sha256 mHash mgfseed_counterLen mgfseed_counter;
+    let acc' = Buffer.sub #uint8 #(v accLen) #(v hLen) acc (mul #SIZE hLen counter) hLen in
+    copy hLen mHash acc'
+  ) st
 
 val mgf_sha256:
-    #len:size_nat ->
-    mgfseed:lbytes (v hLen) ->
-    clen:size_t{v clen == len /\ 0 < len /\ 4 + 2 * v hLen + v hLen * v (blocks clen hLen) < max_size_t} ->
-    res:lbytes len -> Stack unit
-    (requires (fun h -> live h mgfseed /\ live h res /\ disjoint res mgfseed))
-    (ensures (fun h0 _ h1 -> preserves_live h0 h1 /\ modifies1 res h0 h1))
-    [@"c_inline"]
-let mgf_sha256 #len mgfseed clen res =
-    let count_max = blocks clen hLen in
-    let accLen = mul #SIZE hLen count_max in
-    let mgfseed_counter_len = add #SIZE hLen (size 4) in
-    let stLen = add #SIZE (add #SIZE mgfseed_counter_len hLen) accLen in
-    
-    alloc #uint8 #unit #(v stLen) stLen (u8 0) [BufItem mgfseed] [BufItem res]
-    (fun h0 _ h1 -> True)
-    (fun st ->
-       let mgfseed_counter = Buffer.sub #uint8 #(v stLen) #(v mgfseed_counter_len) st (size 0) mgfseed_counter_len in
-       let mgfseed_counter' = Buffer.sub #uint8 #(v mgfseed_counter_len) #(v hLen) mgfseed_counter (size 0) hLen in
-       copy hLen mgfseed mgfseed_counter';
-       //let mHash = Buffer.sub #uint8 #(v stLen) #(v hLen) st mgfseed_counter_len hLen in
-       let acc = Buffer.sub #uint8 #(v stLen) #(v accLen) st (add #SIZE mgfseed_counter_len hLen) accLen in
-       mgf_sha256_ count_max accLen stLen st (size 0);
-       let acc' = Buffer.sub #uint8 #(v accLen) #len acc (size 0) clen in
-       copy clen acc' res
-    )
+  #mgfseedLen:size_nat{mgfseedLen + 4 < max_size_t} -> #maskLen:size_nat ->
+  mmgfseedLen:size_t{v mmgfseedLen = mgfseedLen} -> mgfseed:lbytes mgfseedLen ->
+  mmaskLen:size_t{v mmaskLen = maskLen /\ 0 < maskLen /\ mgfseedLen + 4 + v hLen + v (blocks mmaskLen hLen) * v hLen < pow2 32} ->
+  res:lbytes maskLen -> Stack unit
+  (requires (fun h -> live h mgfseed /\ live h res /\ disjoint res mgfseed))
+  (ensures (fun h0 _ h1 -> preserves_live h0 h1 /\ modifies1 res h0 h1))
+  [@"c_inline"]
+let mgf_sha256 #mgfseedLen #maskLen mmgfseedLen mgfseed mmaskLen res =
+  let count_max = blocks mmaskLen hLen in
+  let accLen = mul #SIZE count_max hLen in
+  let mgfseed_counterLen = add #SIZE mmgfseedLen (size 4) in
+  //st = [mgfseed_counter; hash(mgfseed_counter); acc]
+  let stLen = add #SIZE (add #SIZE mgfseed_counterLen hLen) accLen in
+
+  alloc #uint8 #unit #(v stLen) stLen (u8 0) [BufItem mgfseed] [BufItem res]
+  (fun h0 _ h1 -> True)
+  (fun st ->
+    let mgfseed_counter = Buffer.sub #uint8 #(v stLen) #(v mgfseed_counterLen) st (size 0) mgfseed_counterLen in
+    let mgfseed_st = Buffer.sub #uint8 #(v mgfseed_counterLen) #mgfseedLen mgfseed_counter (size 0) mmgfseedLen in
+    copy mmgfseedLen mgfseed mgfseed_st;
+    mgf_sha256_ #(v stLen) mmgfseedLen accLen stLen st count_max;
+    let acc = Buffer.sub #uint8 #(v stLen) #(v accLen) st (add #SIZE mgfseed_counterLen hLen) accLen in
+    let acc1 = Buffer.sub #uint8 #(v accLen) #maskLen acc (size 0) mmaskLen in
+    copy mmaskLen acc1 res
+  )
